## 1. fn x => x > 1

int -> bool

ここはなんでintになる？


## 2. fn x => fn y => fn z => (x y, x "Ada", y > z)

```
fn x => fn y => fn z => (x  y, x "Ada", y > z)
   t2      t3      t4    _t5_  __t6__  __t7__
                         _________t8_________
________________t1___________________________
```

t1 = t2 -> t3 -> t4 -> t8

t5, t6, t7について

t2 = t3 -> t5
t2 = String -> t6
t7 = bool
t8 = t5 * t6 * t7
t5 = t6
t3 = String

t1 = (string -> t6) -> string -> string -> (t6 * t6 * bool)
   = (string -> 'a) -> string -> string -> ('a * 'a * bool)


## 3. fn x => fn y => y (x > x)

```
fn x  => fn y => y (x > x)
   t1       t2      _t3__
                 ___t4___
___________t5____________
```

t5 = t1 -> t2 -> t4
t2 = t3 -> t4
t3 = bool
t2 = int  
**何も指定がなく四則演算や比較がされている場合勝手にintとする**

t5 = int -> (bool -> 'a) -> 'a
